---
title: "305 Lecture 8.8 - Sampling without Replacement"
author: "Brian Weatherson"
mainfont: SF Pro Rounded
output:
  beamer_presentation:
    md_extensions: +link_attributes+fenced_divs
    keep_tex: yes
    latex_engine: xelatex
    includes:
      in_header: 
        - 305-beamer-header.tex
        - visible-midrule.tex
        - compact-tables.tex
mathfont: STIX Two Math
mainfontoptions: BoldFont = SF Pro Rounded Semibold
---

## Plan

- To illustrate another special kind of updating on two data points: Sampling without Replacement

## Associated Reading

Odds and Ends, Chapter 9

## Dependence

What happens if the events $B_1$ and $B_2$ are dependent on one or other of the hypotheses?

- The typical case is that they will be dependent on none or all of the hypotheses.
- But it's possible in principle to have independence on some and dependence on others. 
- And in that case we have to use the more complicated procedure I'm about to describe.

## Sampling Without Replacement

The paradigm example of conditional dependence is sampling **without replacement**.

- Assume you know which urn I'm using.
- Then the draws without replacement won't be independent because every time you draw a marble, there are fewer marbles of that color to draw the next time.

## Example

Assume that I am using urn A. (Or assume that we are working out conditional probabilities conditional on urn A.)

- For the first draw, the probability of red is 4 in 10, or  0.4.
- Conditional on the first draw being red, the probability of the second draw being red is 3 in 9, or $\frac{1}{3}$.
- That's because there are now 9 marbles left, and 3 of them are red.

## Continuing the Example

So to work out the probability of some sequence of draws $D_1, D_2$ given a hypothesis $X$ about the urn, we need to use the more complicated rule.

$$
\Pr(D_1 \wedge D_2 | X) = \Pr(D_1 | X) \Pr(D_2 | X \wedge D_1)
$$

\pause
For example
$$
\Pr(Red_1 \wedge Red_2 | A) = \Pr(Red_1 | A)\Pr(Red_2 | A \wedge Red_1) = \frac{4}{10} \times \frac{3}{9} = \frac{2}{15}
$$

## Continuing the Example

So to work out the probability of some sequence of draws $D_1, D_2$ given a hypothesis $X$ about the urn, we need to use the more complicated rule.

$$
\Pr(D_1 \wedge D_2 | X) = \Pr(D_1 | X) \Pr(D_2 | X \wedge D_1)
$$

For example
$$
\Pr(Red_1 \wedge Red_2 | B) = \Pr(Red_1 | B)\Pr(Red_2 | B \wedge Red_1) = \frac{8}{10} \times \frac{7}{9} = \frac{28}{45}
$$

## Another Example

There are two urns in front of us.

- One of them - urn A - has 4 red marbles, 3 green marbles, and 3 blue marbles.
- The other - urn B- has 8 red marbles, 1 green marbles and 1 blue marbles. \pause

One of the urns will be selected at random, and then two marbles drawn from it **without replacement**.

- If both draws are red, what is the probability that Urn A was selected?

---

|           |        Red-Red                                               |
|:---------:|:------------------------------------------------------------:|
| Urn A     | $0.5 \times \frac{4}{10} \times \frac{3}{9} = \frac{1}{15}$  |
|           |                                                              |
| Urn B     | $0.5 \times \frac{8}{10} \times \frac{7}{9} = \frac{14}{45}$ |
|           |                                                              |
| **Total** | $\frac{1}{15} + \frac{14}{45} = \frac{17}{45}$               |

\pause
$$
\Pr(A | Red-Red) = \frac{\Pr(A \wedge Red-Red)}{\Pr(Red-Red)} = \frac{\frac{1}{15}}{\frac{17}{45}} = \frac{3}{17}
$$

\bigskip
The probability of Urn A fell by a bit more.

## Yet Another Example

There are two urns in front of us.

- One of them - urn A - has 4 red marbles, 3 green marbles, and 3 blue marbles.
- The other - urn B- has 8 red marbles, 1 green marbles and 1 blue marbles. \pause

One of the urns will be selected at random, and then two marbles drawn from it **with replacement**.

- If the first draw is red and the second green, what is the probability that Urn A was selected?

## The General Conjunction Rule

To work out the probability of some sequence of draws $D_1, D_2$ given a hypothesis $X$ about the urn, we need to use the more complicated rule.
$$
\Pr(D_1 \wedge D_2 | X) = \Pr(D_1 | X) \Pr(D_2 | X \wedge D_1)
$$

\pause
So in this case we get
$$
\Pr(Red_1 \wedge Green_2 | A) = \Pr(Red_1 | A)\Pr(Green_2 | A \wedge Red_1) = \frac{4}{10} \times \frac{3}{9} = \frac{2}{15}
$$

## The General Conjunction Rule

To work out the probability of some sequence of draws $D_1, D_2$ given a hypothesis $X$ about the urn, we need to use the more complicated rule.
$$
\Pr(D_1 \wedge D_2 | X) = \Pr(D_1 | X) \Pr(D_2 | X \wedge D_1)
$$

And for Urn B we get
$$
\Pr(Red_1 \wedge Green_2 | B) = \Pr(Red_1 | B)\Pr(Green_2 | B \wedge Red_1) = \frac{8}{10} \times \frac{1}{9} = \frac{4}{45}
$$

---

|           |        Red-Green                                             |
|:---------:|:------------------------------------------------------------:|
| Urn A     | $0.5 \times \frac{4}{10} \times \frac{3}{9} = \frac{1}{15}$  |
|           |                                                              |
| Urn B     | $0.5 \times \frac{8}{10} \times \frac{1}{9} = \frac{2}{45}$  |
|           |                                                              |
| **Total** | $\frac{1}{15} + \frac{2}{45} = \frac{5}{45}$                 |

\pause
$$
\Pr(A | Red-Green) = \frac{\Pr(A \wedge Red-Green)}{\Pr(Red-Green)} = \frac{\frac{1}{15}}{\frac{5}{45}} = \frac{3}{5}
$$

\bigskip
Which, interestingly, is exactly the same as in the with replacement case.

## For Next Time

We'll end the week with one last example.
